Exhaustive pattern matching on small bit vectors

theories/Bitvector.v
@@ -29,24 +29,41 @@
 From Coq Require Import
      Bool.Bool
      Logic.StrictProp
+     PeanoNat
      NArith.BinNat.
-
+From Equations Require Import
+     Equations.
 From Katamaran Require Import
      Prelude.
 Local Set Implicit Arguments.
-(* Local Set Primitive Projections. *)
+
+Declare Scope bv_scope.
+Delimit Scope bv_scope with bv.
+Declare Scope bv_bitstring_scope.
+Delimit Scope bv_bitstring_scope with bits.
+
+(* Yet another library for sized bitvectors. Ultimately, it would be great to
+   consolidate this with for example: https://github.com/jasmin-lang/coqword or
+   https://github.com/mit-plv/coqutil/tree/master/src/coqutil/Word
+
+   Other resources include:
+   https://github.com/arthuraa/coq-utils/blob/master/theories/word.v
+   https://github.com/mit-plv/bbv
+*)
 
 Module bv.
 
-  Fixpoint at_most (n : nat) {struct n} : positive -> SProp.
-  Proof.
-    destruct n; intros p.
-    - apply sEmpty.
-    - destruct p.
-      + apply (at_most n p).
-      + apply (at_most n p).
-      + apply sUnit.
-  Defined.
+  (* The given [positive] consist of fewer than n bits. *)
+  Fixpoint at_most (n : nat) {struct n} : positive -> SProp :=
+    match n with
+    | O   => fun _ => sEmpty
+    | S n => fun p =>
+               match p with
+               | xI p => at_most n p
+               | xO p => at_most n p
+               | xH => sUnit
+               end
+    end.
 
   Definition is_wf (n : nat) (bs : N) : SProp :=
     match bs with
@@ -54,9 +71,10 @@ Module bv.
     | Npos p => at_most n p
     end.
 
-  Record t (n : nat) : Set :=
-    mk { bin : N; wf : is_wf n bin }.
+  Record bv (n : nat) : Set :=
+    mk { bin : N; _ : is_wf n bin }.
   Arguments mk {n} _ &.
+  Set Transparent Obligations.
 
   Section Conversion.
 
@@ -70,25 +88,32 @@ Module bv.
                 end
       end.
 
-    Lemma wf_double (n : nat) (x : N) :
-      is_wf n x -> is_wf (S n) (N.double x).
-    Proof. destruct x; cbn; intros H; apply H. Qed.
+    Definition wf_double (n : nat) (x : N) :
+      is_wf n x -> is_wf (S n) (N.double x) :=
+       match x with
+       | N0     => fun wf => wf
+       | Npos p => fun wf => wf
+       end.
 
-    Lemma wf_succ_double (n : nat) (x : N) :
-      is_wf n x -> is_wf (S n) (N.succ_double x).
-    Proof. destruct x; cbn; intros H; apply H. Qed.
+    Definition wf_succ_double (n : nat) (x : N) :
+      is_wf n x -> is_wf (S n) (N.succ_double x) :=
+       match x with
+       | N0     => fun wf => wf
+       | Npos p => fun wf => wf
+       end.
 
-    Lemma wf_trunc n : forall p, is_wf n (trunc n p).
-    Proof.
-      induction n; cbn.
-      - constructor.
-      - intros p. destruct p; cbn.
-        + apply wf_succ_double. apply IHn.
-        + apply wf_double. apply IHn.
-        + constructor.
-    Qed.
+    Fixpoint wf_trunc n : forall p, is_wf n (trunc n p) :=
+      match n with
+      | O   => fun _ => stt
+      | S n => fun p =>
+                  match p with
+                  | xI p => wf_succ_double n (trunc n p) (wf_trunc n p)
+                  | xO p => wf_double n (trunc n p) (wf_trunc n p)
+                  | xH   => stt
+                  end
+      end.
 
-    Definition of_N {n} (bs : N) : t n :=
+    Definition of_N {n} (bs : N) : bv n :=
       match bs with
       | N0     => mk N0 stt
       | Npos p => mk (trunc n p) (wf_trunc n p)
@@ -106,8 +131,8 @@ Module bv.
 
   Section Constants.
 
-    Definition zero n : t n := mk 0 stt.
-    Definition one n : t n :=
+    Definition zero n : bv n := mk 0 stt.
+    Definition one n : bv n :=
       match n with
       | 0   => mk 0 stt
       | S _ => mk 1 stt
@@ -115,12 +140,52 @@ Module bv.
 
   End Constants.
 
+  Section NoConfusion.
+
+    Definition NoConfusion_bv {n} (x y : bv n) : Prop :=
+      bin x = bin y.
+
+    Definition noConfusion_bv {n} (x y : bv n) : NoConfusion_bv x y -> x = y :=
+      match x with
+      | mk x p =>
+          match y with
+          | mk y q =>
+              fun e : x = y =>
+                match e in _ = y return forall q : is_wf n y, mk x p = mk y q with
+                | eq_refl => fun q => eq_refl
+                end q
+          end
+      end.
+
+    Definition noConfusion_inv_bv {n} (x y : bv n) : x = y -> NoConfusion_bv x y :=
+      fun e => match e with
+               | eq_refl => eq_refl
+               end.
+
+    #[program]
+    Instance NoConfusionPackage_bv {n} : NoConfusionPackage (bv n) :=
+      {| NoConfusion := @NoConfusion_bv n;
+         noConfusion := @noConfusion_bv n;
+         noConfusion_inv := @noConfusion_inv_bv n;
+      |}.
+    Next Obligation.
+      intros n x y. destruct x as [x p], y as [y q].
+      intros e. change_no_check (x = y) in e.
+      destruct e. reflexivity.
+    Qed.
+    Next Obligation.
+      intros n x y e. destruct e. destruct x. reflexivity.
+    Qed.
+
+  End NoConfusion.
+  Local Existing Instance NoConfusionPackage_bv.
+
   Section Equality.
 
-    Definition eqb {n : nat} (x y : t n) : bool :=
+    Definition eqb {n : nat} (x y : bv n) : bool :=
       N.eqb (bin x) (bin y).
 
-    Lemma eqb_spec {n : nat} : forall (x y : t n), reflect (x = y) (eqb x y).
+    Lemma eqb_spec {n : nat} : forall (x y : bv n), reflect (x = y) (eqb x y).
     Proof.
       intros [x wfx] [y wfy]. unfold eqb. cbn.
       destruct (N.eqb_spec x y); constructor.
@@ -128,39 +193,47 @@ Module bv.
       - now intros p%(f_equal (@bin _)).
     Qed.
 
+    Instance eqdec_bv {n : nat} : EqDec (bv n) :=
+      fun x y =>
+        match eqb_spec x y with
+        | ReflectT _ e => left e
+        | ReflectF _ n => right n
+        end.
+
   End Equality.
+  Local Existing Instance eqdec_bv.
 
   Section Arithmetic.
 
-    Definition add {n} (x y : t n) : t n :=
+    Definition add {n} (x y : bv n) : bv n :=
       of_N (N.add (bin x) (bin y)).
 
-    Definition sub {n} (x y : t n) : t n :=
+    Definition sub {n} (x y : bv n) : bv n :=
       of_N (N.sub (N.shiftl_nat 1 n + bin x) (bin y)).
 
-    Definition mul {n} (x y : t n) : t n :=
+    Definition mul {n} (x y : bv n) : bv n :=
       of_N (N.mul (bin x) (bin y)).
 
   End Arithmetic.
 
   Section Logical.
 
-    Definition land {n} (x y : t n) : t n :=
+    Definition land {n} (x y : bv n) : bv n :=
       of_N (N.land (bin x) (bin y)).
 
-    Definition lor {n} (x y : t n) : t n :=
+    Definition lor {n} (x y : bv n) : bv n :=
       of_N (N.lor (bin x) (bin y)).
 
-    Definition lxor {n} (x y : t n) : t n :=
+    Definition lxor {n} (x y : bv n) : bv n :=
       of_N (N.lxor (bin x) (bin y)).
 
   End Logical.
 
   Section ListLike.
 
-    Definition nil : t 0 :=
+    Definition nil : bv 0 :=
       mk N0 stt.
-    Definition cons [n] (b : bool) (xs : t n) : t (S n) :=
+    Definition cons [n] (b : bool) (xs : bv n) : bv (S n) :=
       match xs with
         mk bs wf =>
           if b
@@ -168,9 +241,9 @@ Module bv.
           else mk (N.double bs) (wf_double n bs wf)
       end.
 
-    Inductive NilView : t 0 -> Set :=
+    Inductive NilView : bv 0 -> Set :=
     | nvnil : NilView nil.
-    Definition nilView (xs : t 0) : NilView xs :=
+    Definition nilView (xs : bv 0) : NilView xs :=
       match xs with
       | mk bs wf =>
           match bs return forall wf : is_wf 0 bs, NilView (mk bs wf) with
@@ -179,15 +252,15 @@ Module bv.
           end wf
       end.
 
-    Inductive ConsView {n} : t (S n) -> Set :=
-    | cvcons (b : bool) (xs : t n) : @ConsView n (cons b xs).
-    Definition consView {n} (xs : t (S n)) : ConsView xs :=
+    Inductive ConsView {n} : bv (S n) -> Set :=
+    | cvcons (b : bool) (xs : bv n) : @ConsView n (cons b xs).
+    Definition consView {n} (xs : bv (S n)) : ConsView xs :=
       match xs with
       | mk bs wf =>
           match bs return forall wf : is_wf (S n) bs, ConsView (mk bs wf) with
           | N0      => fun _ => cvcons false (mk 0 stt)
           | N.pos p =>
-              match p return forall wf : at_most (S n) p, ConsView (mk (N.pos p) wf) with
+              match p with
               | xI p => fun wf => cvcons true  (mk (N.pos p) wf)
               | xO p => fun wf => cvcons false (mk (N.pos p) wf)
               | xH   => fun _  => cvcons true  (mk 0 stt)
@@ -195,20 +268,20 @@ Module bv.
           end wf
       end.
 
-    Inductive View : forall n, t n -> Set :=
+    Inductive View : forall n, bv n -> Set :=
     | isnil  : @View 0 nil
-    | iscons (b : bool) {n} (xs : t n) : @View (S n) (cons b xs).
-    Definition view {n} : forall xs : t n, View xs :=
-      match n return forall xs : t n, View xs with
+    | iscons (b : bool) {n} (xs : bv n) : @View (S n) (cons b xs).
+    Definition view {n} : forall xs : bv n, View xs :=
+      match n return forall xs : bv n, View xs with
       | 0   => fun xs => match nilView xs with nvnil => isnil end
       | S n => fun xs => match consView xs with cvcons b xs => iscons b xs end
       end.
 
-    Definition t_rect (P : forall n : nat, t n -> Type)
+    Definition bv_rect (P : forall n : nat, bv n -> Type)
       (PO : P O nil)
-      (PS : forall n (b : bool) (x : t n), P n x -> P (S n) (cons b x)) :
-      forall [n] (xs : t n), P n xs :=
-      fix t_rect (n : nat) : forall xs : t n, P n xs :=
+      (PS : forall n (b : bool) (x : bv n), P n x -> P (S n) (cons b x)) :
+      forall [n] (xs : bv n), P n xs :=
+      fix t_rect (n : nat) : forall xs : bv n, P n xs :=
         match n with
         | 0   => fun xs => match nilView xs with
                            | nvnil => PO
@@ -220,68 +293,347 @@ Module bv.
 
     Definition fold_right (A : forall n : nat, Type)
       (c : forall n, bool -> A n -> A (S n)) (n : A O) :
-      forall {m} (xs : t m), A m :=
-      t_rect (fun m _ => A m) n (fun m b _ p => c m b p).
+      forall {m} (xs : bv m), A m :=
+      bv_rect (fun m _ => A m) n (fun m b _ p => c m b p).
 
-    Definition app {m n} (xs : t m) (ys : t n) : t (m + n) :=
-      fold_right (fun m => t (m + n)) (fun m => @cons (m + n)) ys xs.
+    Fixpoint fold_left {A : forall n : nat, Type}
+      (c : forall n, A n -> bool -> A (S n)) (n : A O)
+      [m] {struct m} : forall (xs : bv m), A m :=
+      match m with
+      | O    => fun xs =>
+                  match nilView xs with
+                  | nvnil => n
+                  end
+      | S m => fun xs  =>
+                 match consView xs with
+                 | cvcons b xs => fold_left (fun m => c (S m)) (c 0 n b) xs
+                 end
+      end.
+
+    Definition app {m n} (xs : bv m) (ys : bv n) : bv (m + n) :=
+      fold_right (fun m => bv (m + n)) (fun m => @cons (m + n)) ys xs.
     Global Arguments app : simpl never.
 
-    Lemma app_nil {m} (xs : t m) :
+    Lemma app_nil {m} (xs : bv m) :
       app nil xs = xs.
     Proof. reflexivity. Defined.
 
-    Lemma app_cons b {m n} (xs : t m) (ys : t n) :
+    Definition app_cons b {m n} (xs : bv m) (ys : bv n) :
       app (cons b xs) ys = cons b (app xs ys).
     Proof. destruct xs as [[] ?], b; reflexivity. Defined.
 
-    Inductive AppView m n : t (m + n) -> Set :=
-    | isapp (xs : t m) (ys : t n) : AppView _ _ (app xs ys).
+    Inductive AppView m n : bv (m + n) -> Set :=
+    | isapp (xs : bv m) (ys : bv n) : AppView _ _ (app xs ys).
 
-    Definition avcons {m n} b {xs} (axs : AppView m n xs) : AppView (S m) n (cons b xs).
-    Proof. destruct axs. rewrite <- app_cons. constructor. Defined.
+    Import EqNotations.
+    Definition avcons {m n} b {xs} (axs : AppView m n xs) :
+      AppView (S m) n (cons b xs) :=
+      match axs with
+      | isapp xs ys => rew app_cons b xs ys in isapp (cons b xs) ys
+      end.
 
-    Fixpoint appView m n {struct m} : forall xs : t (m + n), AppView _ _ xs.
-      destruct m; cbn [plus].
-      - apply (@isapp 0 n nil).
-      - intros xs. destruct (consView xs). apply avcons. apply appView.
-    Defined.
+    Fixpoint appView m n {struct m} : forall xs : bv (m + n), AppView _ _ xs :=
+      match m with
+      | O   => isapp nil
+      | S m => fun xs =>
+                 match consView xs with
+                 | cvcons b xs => avcons b (appView m n xs)
+                 end
+      end.
+
+    Definition rev_append {m n} (x : bv m) (y : bv n) : bv (m + n) :=
+      fold_left (A := fun k => bv (k + n)) (fun k (z : bv (k + n)) b => cons b z) y x.
+    Definition rev {m} (x : bv m) : bv m :=
+      fold_left (fun k (z : bv k) b => cons b z) nil x.
+
+    Lemma cons_inj [n] (x y : bool) (xs ys : bv n) :
+      cons x xs = cons y ys -> x = y /\ xs = ys.
+    Proof.
+      destruct xs as [xs wfxs], ys as [ys wfys], x, y; intros Heq.
+      - split; auto.
+        apply noConfusion_inv in Heq.
+        apply N.succ_double_inj in Heq.
+        destruct Heq. reflexivity.
+      - exfalso. apply noConfusion_inv in Heq.
+        destruct xs, ys; discriminate Heq.
+      - exfalso. apply noConfusion_inv in Heq.
+        destruct xs, ys; discriminate Heq.
+      - split; auto.
+        apply noConfusion_inv in Heq.
+        apply N.double_inj in Heq.
+        destruct Heq. reflexivity.
+    Qed.
 
   End ListLike.
 
-  Module rec.
+  Section Finite.
 
-    Fixpoint t (n : nat) : Set :=
-      match n with
-      | O   => unit
-      | S n => bool * t n
+    Fixpoint enumV {V : forall k : nat, Type} (c : forall k, bool -> V k -> V (S k))
+      (n : V O) (m : nat) {struct m} : list (V m) :=
+      match m with
+      | O   => Datatypes.cons n Datatypes.nil
+      | S m => Datatypes.app
+                 (enumV (fun k => c (S k)) (c O false n) m)
+                 (enumV (fun k => c (S k)) (c O true n) m)
       end.
 
-    Definition nil : t 0 := tt.
-    Definition cons [n] (b : bool) (xs : t n) : t (S n) := (b , xs).
+    Lemma enumV_length {V : forall k : nat, Type} (c : forall k, bool -> V k -> V (S k)) (n : V O) (m : nat) :
+      length (enumV c n m) = 2 ^ m.
+    Proof.
+      revert V c n. induction m; intros V c n.
+      - reflexivity.
+      - specialize (IHm (fun k => V (S k)) (fun k => c (S k))).
+        cbn. now rewrite List.app_length, !IHm, Nat.add_0_r.
+    Qed.
 
-    Definition t_rect (P : forall n : nat, t n -> Type)
-      (PO : P O nil)
-      (PS : forall n (b : bool) (x : t n), P n x -> P (S n) (cons b x)) :
-      forall [n] (x : t n), P n x :=
-      fix t_rect (n : nat) : forall x : t n, P n x :=
-        match n with
-        | 0   => fun x => match x with tt    => PO end
-        | S n => fun x => match x with (b,x) => PS n b x (t_rect n x) end
-        end.
+    Lemma enumV_inj {V : forall k : nat, Type} (c : forall k, bool -> V k -> V (S k))
+      (c_inj : forall k b1 b2 v1 v2, c k b1 v1 = c k b2 v2 -> b1 = b2 /\ v1 = v2)
+      (n1 n2 : V O) (m : nat) :
+      enumV c n1 m = enumV c n2 m -> n1 = n2.
+    Proof.
+      revert V c c_inj n1 n2. induction m; intros V c c_inj n1 n2.
+      - intros H%noConfusion_inv%(f_equal pr1). exact H.
+      - cbn [enumV]. intros [H1 H2]%list.app_inj_1.
+        apply (IHm (fun k => V (S k)) (fun k => c (S k))) in H1.
+        + now apply c_inj in H1.
+        + intros k. apply c_inj.
+        + do 2 rewrite (@enumV_length (fun k => V (S k))).
+          reflexivity.
+    Qed.
 
-    Definition fold_right (A : forall n : nat, Type)
-      (c : forall n, bool -> A n -> A (S n)) (n : A O) :
-      forall {m} (xs : t m), A m :=
-      t_rect (fun m _ => A m) n (fun m b _ p => c m b p).
+    Lemma enumV_disjoint {V : forall k : nat, Type} (c : forall k, bool -> V k -> V (S k))
+      (c_inj : forall k b1 b2 v1 v2, c k b1 v1 = c k b2 v2 -> b1 = b2 /\ v1 = v2)
+      (n1 n2 : V O) (Heq : n1 <> n2) (m : nat) :
+      forall (x : V m),
+        base.elem_of_list x (enumV c n1 m) ->
+        base.elem_of_list x (enumV c n2 m) -> False.
+    Proof.
+      revert V c c_inj n1 n2 Heq. induction m; intros V c c_inj n1 n2 Heq; cbn [enumV].
+      - intros x xIn1%list.elem_of_list_singleton xIn2% list.elem_of_list_singleton.
+        congruence.
+      - specialize (IHm (fun k => V (S k)) (fun k => c (S k)) (fun k => c_inj (S k))).
+        intros x [in1|in1]%list.elem_of_app [in2|in2]%list.elem_of_app;
+          refine (IHm _ _ _ x in1 in2); intros []%c_inj; congruence.
+    Qed.
 
-  End rec.
+    Lemma nodup_enumV {V : forall k : nat, Type} (c : forall k, bool -> V k -> V (S k))
+      (c_inj : forall k b1 b2 v1 v2, c k b1 v1 = c k b2 v2 -> b1 = b2 /\ v1 = v2)
+      (n : V O) (m : nat) : base.NoDup (enumV c n m).
+    Proof.
+      revert V c c_inj n. induction m; intros V c c_inj n; cbn [enumV].
+      - apply list.NoDup_singleton.
+      - specialize (IHm (fun k => V (S k)) (fun k => c (S k)) (fun k => c_inj (S k))).
+        apply list.NoDup_app. repeat apply conj; auto.
+        cbv - [enumV]. intros x.
+        apply (@enumV_disjoint (fun k => V (S k)) (fun k => c (S k)) (fun k => c_inj (S k))).
+        intros []%c_inj; congruence.
+    Qed.
 
-  Definition to_rec {n} : t n -> rec.t n :=
-    fold_right rec.t rec.cons rec.nil.
+    Lemma elem_of_enumV {V : forall k : nat, Type} (c : forall k, bool -> V k -> V (S k)) (n : V O) (m : nat) :
+      forall (b : bool) (x : V m),
+        base.elem_of x (enumV c n m) ->
+        base.elem_of (c m b x) (enumV c n (S m)).
+    Proof.
+      revert V c n. induction m; cbn; intros V c n b x xIn.
+      - apply list.elem_of_list_singleton in xIn. subst x.
+        destruct b; repeat constructor.
+      - rewrite ?list.elem_of_app. rewrite list.elem_of_app in xIn.
+        destruct xIn as [xIn|xIn];
+          specialize (IHm (fun k => V (S k)) (fun k => c (S k)) _ b _ xIn);
+          cbn in IHm; rewrite list.elem_of_app in IHm; intuition.
+    Qed.
 
-  Definition of_rec {n} : rec.t n -> t n :=
-    rec.fold_right t cons nil.
+    Definition enum (n : nat) : list (bv n) :=
+      enumV cons nil n.
+
+    Lemma nodup_enum (n : nat) : base.NoDup (enum n).
+    Proof. apply (nodup_enumV cons (@cons_inj)). Qed.
+
+    Lemma elem_of_enum (m : nat) (x : bv m) : base.elem_of x (enum m).
+    Proof.
+      induction x using bv_rect.
+      - now apply list.elem_of_list_singleton.
+      - now apply elem_of_enumV.
+    Qed.
+
+    Instance finite_bv {n} : finite.Finite (bv n) :=
+      {| stdpp.finite.enum         := enum n;
+         stdpp.finite.NoDup_enum   := nodup_enum n;
+         stdpp.finite.elem_of_enum := @elem_of_enum n;
+      |}.
+
+  End Finite.
+
+  (* Big-endian bit strings (radix 2 strings). This type is defined by recursion
+     over the number of bits and is less efficient than the subtype
+     representation. The intended use case is exhaustive pattern matching over
+     small bit vectors, i.e. up to ~7-8 bits. It can also be used to define
+     constants of medium sized bit vectors (256-bits or so), but should be
+     avoided for large bit vectors. *)
+  Module bitstring.
+
+    Local Set Transparent Obligations.
+
+    (* A raw representation of bit string intended for the definition of the
+       number notation. *)
+    Inductive raw : Set := rI (_:raw) | rO (_:raw) | rN.
+    Inductive null : Set := bN.
+    Derive NoConfusion EqDec for null.
+
+    Section Digit.
+      Context {A : Set} {eqA : EqDec A}.
+      Inductive digit : Set :=
+      | bO (_:A) | bI (_:A).
+      Derive NoConfusion EqDec for digit.
+    End Digit.
+    Global Arguments digit : clear implicits.
+
+    (* Parse a decimal number into a raw bit string, failing if any digit other
+       than 0 or 1 is used. This doesn't check the length of the decimal. *)
+    Definition of_uint (u : Number.uint) : option raw :=
+      let fix f (u : Decimal.uint) : option raw :=
+        match u with
+        | Decimal.Nil  => Some rN
+        | Decimal.D0 u => option_map rO (f u)
+        | Decimal.D1 u => option_map rI (f u)
+        | _ => None
+        end
+      in match u with
+         | Number.UIntDecimal u => f u
+         | Number.UIntHexadecimal _ => None
+         end.
+
+    (* Unparse the given raw bit string. *)
+    Definition to_uint (r : raw) : Number.uint :=
+      let fix f (r : raw) : Decimal.uint :=
+        match r with
+        | rI r => Decimal.D1 (f r)
+        | rO r => Decimal.D0 (f r)
+        | rN   => Decimal.Nil
+        end
+      in Number.UIntDecimal (f r).
+
+  End bitstring.
+
+  Fixpoint bitstring (n : nat) : Set :=
+    match n with
+    | O   => bitstring.null
+    | S n => bitstring.digit (bitstring n)
+    end.
+
+  Fixpoint bitstring_zeroes (n : nat) : bitstring n :=
+    match n with
+    | O   => bitstring.bN
+    | S n => bitstring.bO (bitstring_zeroes n)
+    end.
+
+  Fixpoint fold_left_nat {A : forall n : nat, Type}
+    (s : forall n, A n -> A (S n)) (z : A O) (m : nat) {struct m} : A m :=
+    match m as n return (A n) with
+    | O   => z
+    | S n => fold_left_nat (fun k => s (S k)) (s 0 z) n
+    end.
+
+  Fixpoint fold_left_positive {A : forall n : nat, Type}
+    (cI : forall n, A n -> A (S n))
+    (cO : forall n, A n -> A (S n))
+    (n : A O) {m : nat} (p : positive) {struct m} : A m :=
+    match m with
+    | O => n
+    | S m =>
+        match p with
+        | xI p => fold_left_positive (fun k => cI (S k)) (fun k => cO (S k)) (cI 0 n) p
+        | xO p => fold_left_positive (fun k => cI (S k)) (fun k => cO (S k)) (cO 0 n) p
+        | xH   => fold_left_nat (fun k => cO (S k)) (cI 0 n) m
+        end
+    end.
+
+  (* The subtype representation is little-endian while bitstring are big-endian.
+     So use a fold-left to reverse the order *)
+  Definition to_bitstring {n} (x : bv n) : bitstring n :=
+    match x with
+    | mk N0 _        => bitstring_zeroes n
+    | mk (N.pos p) _ => fold_left_positive
+                          (fun k => @bitstring.bI (bitstring k))
+                          (fun k => @bitstring.bO (bitstring k))
+                          bitstring.bN p
+    end.
+
+  Fixpoint fold_bitstring_left {A : forall k : nat, Type}
+    (c : forall k, A k -> bool -> A (S k)) (n : A O)
+    [m] {struct m} : forall (xs : bitstring m), A m :=
+    match m with
+    | O   => fun _ => n
+    | S m =>
+        fun xs =>
+          match match xs with
+                | bitstring.bO a => (false,a)
+                | bitstring.bI a => (true,a)
+                end with
+          | (b,a) =>
+              fold_bitstring_left (fun k => c (S k)) (c 0 n b) a
+          end
+    end.
+
+  Definition of_bitstring : forall n, bitstring n -> bv n :=
+    fold_bitstring_left (A := bv) (fun _ x b => cons b x) nil.
+
+  Arguments to_bitstring [n] & _%bv.
+  Arguments of_bitstring [n] & _%bits.
+
+  Module notations.
+    Open Scope bv_scope.
+    Open Scope bv_bitstring_scope.
+
+    (* Coq doesn't like the fixpoint definition of bitstrings. Squelch the
+       warnings. *)
+    Local Set Warnings "-via-type-mismatch -via-type-remapping".
+
+    (* Number notation for bitstrings. This is a combination of the "Number
+       Notation for radix 3" and "Number Notation with implicit arguments"
+       examples given in
+       https://coq.inria.fr/refman/user-extensions/syntax-extensions.html#number-notations
+    *)
+    Number Notation bitstring bitstring.of_uint bitstring.to_uint
+           (via bitstring.raw mapping
+                [[bitstring.bI] => bitstring.rI,
+                 [bitstring.bO] => bitstring.rO,
+                 [bitstring.bN] => bitstring.rN]) : bv_bitstring_scope.
+
+    (* The number notation does not work for printing patterns in pattern
+       matches, but curiously works for parsing. Possibly due to the via-type
+       remappings whose warnings we silenced above. As a workaround we define
+       printing only notations for the constructors that achieve the same result
+       as printing the number notation. *)
+    Notation "" := (bitstring.bN)
+      (at level 0, right associativity, only printing) : bv_bitstring_scope.
+    Notation "1 b" := (bitstring.bI b)
+      (at level 0, right associativity, format "1 b", only printing) : bv_bitstring_scope.
+    Notation "0 b" := (bitstring.bO b)
+      (at level 0, right associativity, format "0 b", only printing) : bv_bitstring_scope.
+
+    Notation "[ 'bits' x ]" := (of_bitstring x%bits)
+      (format "[ 'bits'  x ]") : bv_scope.
+    Notation "[ 'bits' ]" := (@of_bitstring 0 bitstring.bN)
+      (format "[ 'bits' ]") : bv_scope.
+    Notation "[ 'bits' [ n ] x ]" := (@of_bitstring n x%bits)
+      (only parsing) : bv_scope.
+    Notation "[ 'bits' [ 0 ] ]" := (@of_bitstring 0 bitstring.bN)
+      (only parsing) : bv_scope.
+
+    Notation "[ 'bv' x ]" := (mk x%xN stt) (format "[ 'bv'  x ]") : bv_scope.
+    Notation "[ 'bv' [ n ] x ]" := (@mk n x%xN stt) (only parsing) : bv_scope.
+
+  End notations.
 
 End bv.
-Notation bv n := (bv.t n).
+Export bv (bv).
+
+Bind Scope bv_scope with bv.
+Bind Scope bv_bitstring_scope with bv.bitstring.
+Bind Scope bv_bitstring_scope with bv.bitstring.null.
+Bind Scope bv_bitstring_scope with bv.bitstring.digit.
+
+#[export] Existing Instance bv.NoConfusionPackage_bv.
+#[export] Existing Instance bv.eqdec_bv.
+#[export] Existing Instance bv.finite_bv.
